Sep_Main.thy
@@ -1,7 +1,7 @@
 theory Sep_Main
   imports
-    "SepLogicTime_RBTreeBasic.SepAuto" 
-  SepLog_Automatic
+    "SepLogicTime_RBTreeBasic.SepAuto_Time" 
+  "SepAuto_Time.SepLog_Automatic"
 begin
 
 end
